Prove that the example typechecks

Example.v
@@ -1,44 +1,191 @@
-Require Import Fsub_Definitions.
-Require Import Fsub_Infrastructure.
+Require Import Fsub_Lemmas.
 
 Check (exp_abs (typ_capt cset_universal typ_top) 0).
 Check (typ_arrow (typ_capt cset_universal typ_top)
-                  (typ_capt (cset_set {} (NatSet.F.singleton 0)) typ_top)).
+                 (typ_capt (cset_set {} (NatSet.F.singleton 0)) typ_top)).
 
-Lemma ezy_pzy_lemon_sqzy :
-   typing empty
-          (exp_abs (typ_capt cset_universal typ_top) 0)
-          (typ_capt {}C
-                    (typ_arrow (typ_capt cset_universal typ_top)
-                               (typ_capt (cset_set {}
-                                (NatSet.F.singleton 0)) typ_top)))
+Ltac hint := trivial.
+Ltac hint ::=
+  eauto.
+Ltac fnset_mem_dec :=
+  symmetry; rewrite <- NatSetFacts.mem_iff; fsetdec.
+
+Set Nested Proofs Allowed.
+Lemma cset_eq_injectivity : forall a1 a2 n1 n2,
+    a1 = a2 ->
+    n1 = n2 ->
+    cset_set a1 n1 = cset_set a2 n2.
+Proof.
+  intros *. intros EqA EqN.
+  rewrite EqA.
+  rewrite EqN.
+  trivial.
+Qed.
+
+Ltac cset_eq_dec :=
+  apply cset_eq_injectivity; [try fsetdec | try fnsetdec].
+
+Ltac replace_if_cond_with val tac :=
+  match goal with
+  | _ :_ |- context[if ?c then _ else _] =>
+    replace c with val by tac
+  end.
+
+Ltac replace_if_cond_with_left :=
+  let e := fresh "e" in
+  let Eq := fresh "Eq" in
+  let P := fresh "P" in
+  match goal with
+  |- context[if ?c then _ else _] =>
+  assert (exists v, c = left v) as Eq; [
+    destruct c as [P | P];
+    (contradiction ||
+     inversion P;
+     eexists;
+     reflexivity) |
+    destruct Eq as [e Eq];
+    rewrite Eq;
+    clear Eq;
+    clear e
+  ]
+  end.
+
+Ltac simpl_hammer :=
+  repeat (unfold open_tt, open_tpt, open_te, open_ee, open_ct, open_cpt, open_cset,
+          binds
+          ; simpl).
+
+(* Ltac clear_frees := *)
+(*   repeat match goal with *)
+(*          | H : _ `notin` _ |- _ => *)
+(*            clear H *)
+(*          end. *)
+
+(* Hint Extern 10 (AtomSet.F.Subset _ _) => *)
+(* idtac "go fsetdec go" ; *)
+(* (* NOTE: "free" hypothesis are unlikely to help with subsets and they can cause fsetdec to hang *) *)
+(* try solve [clear_frees; simpl_env in *; fsetdec] *)
+(* : core. *)
+
+Fixpoint dom_typ (E : list (atom * binding)) : atoms :=
+  match E with
+  | nil => AtomSet.F.empty
+  | (x, bind_typ _) :: E' => AtomSet.F.union (singleton x) (dom_typ E')
+  | (x, bind_sub _) :: E' => (dom_typ E')
+  end.
+
+Ltac prepare_for_fsetdec ::=
+  clear_frees; simpl_env in *; simpl dom_typ in *.
+
+Lemma dom_typ_subsets_dom : forall E,
+    AtomSet.F.Subset (dom_typ E) (dom E).
+Proof.
+  induction E.
+  - simpl_hammer; fsetdec.
+  - simpl_hammer.
+    destruct a as [a b].
+    destruct b; fsetdec.
+Qed.
+
+Lemma allbound_typ_if : forall E A,
+  ok E ->
+  AtomSet.F.Subset A (dom_typ E) ->
+  allbound_typ E A.
+Proof.
+  intros.
+  unfold allbound_typ.
+  generalize dependent A.
+  induction E; intros.
+  - simpl dom_typ in *.
+    assert (x `in` {}) by fsetdec.
+    rewrite AtomSetFacts.empty_iff in H2.
+    contradiction.
+  - simpl dom_typ in *.
+    destruct a.
+    destruct b.
+    + simpl_hammer.
+      destruct (x == a).
+      * exfalso.
+        inversion H; subst.
+        pose proof (dom_typ_subsets_dom E).
+        assert (a `in` dom E) as P by fsetdec.
+        apply (H6 P).
+      * inversion H; subst.
+        apply IHE with (A := A); trivial.
+    + simpl_hammer.
+      destruct (x == a).
+      * eauto.
+      * inversion H; subst.
+        assert (x `in` dom_typ E) by fsetdec.
+        apply IHE with (A := dom_typ E); eauto.
+Qed.
+
+Lemma ezy_pzy_lemon_sqzy : forall E,
+  wf_env E ->
+  typing E
+         (exp_abs (typ_capt cset_universal typ_top) 0)
+         (typ_capt {}C
+                   (typ_arrow (typ_capt cset_universal typ_top)
+                              (typ_capt (cset_set {} (NatSet.F.singleton 0)) typ_top)))
 .
 Proof with eauto.
-   pick fresh x and apply typing_abs.
-   - simpl.
-     Hint Unfold open_ee : core.
-     Hint Unfold open_ct : core.
-     Hint Unfold open_cset : core.
-     repeat (unfold open_tt, open_tpt, open_te, open_ee, open_ct,
-open_cpt, open_cset; simpl).
-     Check (NatSet.F.mem 0 (NatSet.F.singleton 0)).
-     replace (NatSet.F.mem 0 (NatSet.F.singleton 0)) with true.
-     2 : admit.
-     replace (cset_set (singleton x `union` {})
-                       (NatSet.F.union {}N (NatSet.F.remove 0
-(NatSet.F.singleton 0))))
-       with (x : captureset).
-     apply typing_var with (C := cset_universal).
-     + econstructor...
-     + unfold binds.
-       simpl.
-       assert (x = x) as COME_ON by trivial.
-       assert ((x == x) = (inl COME_ON : {x = x} + {x <> x})).
-       replace  with .
-       Check (x == x).
-       Locate "_ == _".S
-       Locate "_ + _".
-       sum
-       eq_atom_dec
-       atoms
-       replace (x == x) with {x = x}.
+  intros.
+  pick fresh x and apply typing_abs.
+  - simpl_hammer.
+    replace_if_cond_with true fnset_mem_dec.
+    replace (cset_set (singleton x `union` {})
+                      (NatSet.F.union {}N (NatSet.F.remove 0 (NatSet.F.singleton 0))))
+      with (cset_fvar x)
+      by cset_eq_dec.
+    apply typing_var with (C := cset_universal).
+    + econstructor...
+    + simpl_hammer;
+        replace_if_cond_with_left...
+  - pick fresh x and apply wf_typ_arrow...
+    simpl_hammer.
+    replace_if_cond_with true fnset_mem_dec.
+    replace (cset_set (singleton x `union` {})
+                      (NatSet.F.union {}N (NatSet.F.remove 0 (NatSet.F.singleton 0))))
+      with (cset_fvar x)
+      by cset_eq_dec.
+    apply wf_typ_capt...
+    eapply wf_concrete_cset...
+    apply allbound_typ_if...
+Qed.
+
+
+Lemma ez_pz_lemon_sqz :
+  typing empty
+         (exp_tabs (typ_capt cset_universal typ_top)
+                   (exp_abs (typ_capt cset_universal typ_top)
+                            0))
+         (typ_capt {}C
+                   (typ_all (typ_capt cset_universal typ_top)
+                            (typ_capt {}C
+                                      (typ_arrow (typ_capt cset_universal typ_top)
+                                                 (typ_capt (cset_set {} (NatSet.F.singleton 0))
+                                                           typ_top)))))
+.
+Proof with eauto.
+  pick fresh X and apply typing_tabs.
+  - simpl_hammer.
+    apply ezy_pzy_lemon_sqzy.
+    econstructor...
+  - pick fresh X and apply wf_typ_all...
+    simpl_hammer.
+    apply wf_typ_capt... {
+      eapply wf_concrete_cset...
+      apply allbound_typ_if...
+    }
+    (* just copied from above... *)
+    pick fresh x and apply wf_typ_arrow...
+    simpl_hammer.
+    replace_if_cond_with true fnset_mem_dec.
+    replace (cset_set (singleton x `union` {})
+                      (NatSet.F.union {}N (NatSet.F.remove 0 (NatSet.F.singleton 0))))
+      with (cset_fvar x)
+      by cset_eq_dec.
+    apply wf_typ_capt...
+    eapply wf_concrete_cset...
+    apply allbound_typ_if...
+Qed.
